fr.inria.atlanmod.coqtl.coq/core/Certification.v
@@ -337,28 +337,34 @@ Section Certification.
   (**- crush.
   Qed.**)
 
-  Instance CoqTLEngine :
-    TransformationEngine tc:=
+  Instance CoqTLSyntax :
+    TransformationSyntax tc :=
     {
-      (* syntax and accessors *)
+        (* syntax and accessors *)
 
-      Transformation := Transformation;
-      Rule := Rule;
-      OutputPatternElement := OutputPatternElement;
-      OutputPatternElementReference := OutputPatternElementReference;
+        Transformation := Transformation;
+        Rule := Rule;
+        OutputPatternElement := OutputPatternElement;
+        OutputPatternElementReference := OutputPatternElementReference;
 
-      TraceLink := TraceLink;
+        TraceLink := TraceLink;
 
-      Transformation_getRules := Transformation_getRules;
+        Transformation_getArity := Transformation_getArity;
+        Transformation_getRules := Transformation_getRules;
 
-      Rule_getOutputPatternElements := Rule_getOutputPatternElements;
+        Rule_getOutputPatternElements := Rule_getOutputPatternElements;
 
-      OutputPatternElement_getOutputElementReferences := OutputPatternElement_getOutputElementReferences;
+        OutputPatternElement_getOutputElementReferences := OutputPatternElement_getOutputElementReferences;
 
-      TraceLink_getSourcePattern := TraceLink_getSourcePattern;
-      TraceLink_getIterator := TraceLink_getIterator;
-      TraceLink_getName := TraceLink_getName;
-      TraceLink_getTargetElement := TraceLink_getTargetElement;
+        TraceLink_getSourcePattern := TraceLink_getSourcePattern;
+        TraceLink_getIterator := TraceLink_getIterator;
+        TraceLink_getName := TraceLink_getName;
+        TraceLink_getTargetElement := TraceLink_getTargetElement;      
+    }.
+
+  Instance CoqTLEngine :
+    TransformationEngine CoqTLSyntax :=
+    {
 
       (* semantic functions *)
 
